\documentclass[11pt]{article}
\usepackage{amsfonts,amsmath,amssymb,amsthm,graphicx}
\usepackage{multirow}
\usepackage{booktabs}
\usepackage[caption=false]{subfig} 
\usepackage{color}
\usepackage{ifthen}

\setlength{\topmargin}{0 mm}
\setlength{\oddsidemargin}{5 mm}
\setlength{\evensidemargin}{5 mm}
\setlength{\textwidth}{150 mm}
\setlength{\textheight}{210 mm}

\include{macros}

\begin{document}

\title{Notes on Schr\"odinger's equation}

\author{N. Anders Petersson\thanks{Center for Applied
    Scientific Computing, Lawrence Livermore National Laboratory, L-561, PO Box 808, Livermore CA
    94551. }}

\date{\today}

\maketitle

\section{Eigenfunctions of the continuous problem}
 Consider the 1-D Schr\"odinger equation governing the wave function $\Psi(x,t)$,
\begin{equation}\label{eq_shrodinger-time}
i\hbar\frac{\p \Psi}{\p t} = -\frac{\hbar^2}{2 m} \frac{\p^2}{\p x^2} \Psi + V(x) \Psi,\quad t\geq
0,\quad \| \Psi \| < \infty
\end{equation}
subject to appropriate initial conditions. Here, $V(x)$ is a potential function. For a harmonic
oscillator, the potential function satisfies
\[
V(x) = \frac{1}{2}m\omega^2 x^2.
\]
We can solve \eqref{eq_shrodinger-time} using separation of variables. We make the ansatz
\[
\Psi(x,t) = \phi(t) \psi(x),
\]
which we insert into \eqref{eq_shrodinger-time}. In the standard way, we obtain
\begin{equation} \label{eq_const-ratio}
e:= \frac{i\hbar \phi'}{\phi} = \frac{1}{\psi} \left(-\frac{\hbar^2}{2m} \frac{\p^2\psi}{\p x^2} +
\frac{1}{2} m \omega^2 x^2 \psi \right).
\end{equation}
Because $\phi=\phi(t)$ and $\psi=\psi(x)$, the coefficient $e$ must be constant for all $x$ and
$t$. This observation leads to the eigenvalue problem
\begin{equation}\label{eq_eigen-problem}
e\psi = -\frac{\hbar^2}{2m} \frac{\p^2\psi}{\p x^2} + \frac{1}{2} m \omega^2 x^2 \psi := \hat{H}\psi.
\end{equation}
Here, $e$ is the eigenvalue, $\psi$ is the eigenfunction, and $\hat{H}$ is called the Hamiltonian
operator. The right hand side can be factored according to
\[
\hat{H}\psi = \frac{\hbar\omega}{2}
%
\left(\sqrt{\frac{m\omega}{\hbar}} x - \frac{\hbar}{\sqrt{m\omega}} \frac{\p}{\p x} \right)
%
\left(\sqrt{\frac{m \omega}{\hbar}} x + \frac{\hbar}{\sqrt{m\omega}} \frac{\p}{\p x} \right) \psi +
%
\frac{\hbar \omega}{2} \psi.
\]
Thus, the Hamiltonian operator can written as
\begin{equation}\label{eq_ladder}
\hat{H}\psi = \hbar\omega\left( a^\dag a + \frac{1}{2} I\right)\psi,
\end{equation}
where we have introduced the lowering operator $a$,
\begin{equation}
  a = \frac{1}{\sqrt{2}} \left(\frac{x}{x_0} + x_0 \frac{\p}{\p x} \right),\quad x_0 = \sqrt{\frac{\hbar}{m\omega}},
\end{equation}
and its adjoint, the raising operator, $a^\dag$,
\begin{equation}
  a^\dag= \frac{1}{\sqrt{2}} \left(\frac{x}{x_0} - x_0 \frac{\p}{\p x} \right).
\end{equation}

The factorization of the Hamiltonian operator allows the eigenvalues and eigenfunctions to be
computed in a very elegant way. The fundamental eigenfunction corresponds to the ground state and is
denoted $\psi_0(x)$. It satisfies
\[
a \psi_0 = 0.
\]
This equation is solved by the normalized Gaussian function
\[
\psi_0(x) = \frac{e^{-x^2/(2 x_0^2)}}{\pi^{1/4} x_0^{1/2}},\quad \int_{-\infty}^\infty |\psi_0|^2 \,
dx = 1.
\]
The corresponding eigenvalue follows from \eqref{eq_ladder},
\[
\hat{H}\psi_0 = \hbar\omega\left( a^\dag a + \frac{1}{2}I \right)\psi_0 = \frac{\hbar\omega}{2}
\psi_0,\quad e_0 = \frac{\hbar\omega}{2}.
\]

To derive the higher eigenfunctions, we start by studying the commutator
\begin{equation}\label{eq_a-commut}
[a,a^\dag] = a a^\dag - a^\dag a = \ldots = I.
\end{equation}
Therefore,
\[
  [\hat{H}a^\dag] = \hat{H}a^\dag - a^\dag \hat{H} = \hbar\omega(a^\dag a a^\dag - a^\dag a^\dag a) =
%
  \hbar\omega a^\dag[a,a^\dag] =   \hbar\omega a^\dag.
\]
We conclude that
\begin{equation}\label{eq_comm-rel}
\hat{H} a^\dag = a^\dag \hat{H} +  \hbar\omega a^\dag.
\end{equation}

Assume we know the normalized eigenfunction $\psi_n(x)$ with eigenvalue $e_n$. From
\eqref{eq_comm-rel},
\[
\hat{H} a^\dag\psi_n = a^\dag \hat{H} \psi_n + \hbar\omega a^\dag \psi_n = (e_n + \hbar\omega)
a^\dag \psi_n.
\]
We conclude that $a^\dag\psi_n$ is an (unnormalized) eigenfunction with
eigenvalue $e_{n+1} = e_n + \hbar\omega$. We write the normalized eigenfunction as
$\psi_{n+1} = \beta^{-1} a^\dag \psi_n$, where the normalization factor $\beta$ will be determined below.
Because $\psi_0$ has eigenvalue $e_0 = \hbar\omega/2$,
\begin{align*}
  e_1 &= e_0 + \hbar\omega = \hbar\omega\left( 1+\frac{1}{2} \right),\\
  e_2 &= e_1 + \hbar\omega = e_0 + 2\hbar\omega = \left( 2 + \frac{1}{2} \right),\\
  &\vdots\\
  e_n &= \hbar\omega\left( n + \frac{1}{2} \right),\quad n=0,1,2,\ldots.
\end{align*}
From the definition of the eigenvalue problem \eqref{eq_eigen-problem} and the factorization
\eqref{eq_ladder},
\[
\hbar\omega\left( a^\dag a + \frac{1}{2}I \right)\psi_n = e_n \psi_n = \hbar\omega\left( n +
\frac{1}{2} \right)\psi_n. 
\]
We define the number operator by
\begin{equation}\label{eq_numer-op}
\hat{N} = a^\dag a.
\end{equation}
It has the same eigenfunctions as $\hat{H}$ and non-negative integer eigenvalues,
\[
\hat{N}\psi_n = n \psi_n,\quad n=0,1,2,\ldots
\]

To normalize the eigenfunction $\psi_{n+1}(x) = \beta^{-1} a^\dag \psi_n$, we start by defining $u(x) =
a^\dag\psi_n(x)$. Its norm is defined by
\[
\| u \|^2 = \langle u, u \rangle = \int_{-\infty}^\infty \bar{u}(x) u(x)\, dx.
\]
From the definition of the adjoint of an operator,
\[
\langle a^\dag\psi_n, a^\dag\psi_n\rangle = \langle \psi_n, a a^\dag \psi_n \rangle
\]
From \eqref{eq_a-commut} and \eqref{eq_numer-op}, $a a^\dag = \hat{N} + I$. Therefore,
\[
\langle a^\dag\psi_n, a^\dag\psi_n\rangle = \langle \psi_n, (\hat{N}+I)\psi_n \rangle = (n+1) \| \psi_n \|^2.
\]
Because $\| \psi_n \|=1$, the normalized eigenfunction becomes
\begin{equation}\label{eq_eigenfunction-recursive}
\psi_{n+1}(x) = \frac{1}{\sqrt{n+1}} a^\dag\psi_n(x),\quad n=0,1,2,\ldots.
\end{equation}
This relation can also be written
\[
\sqrt{n+1}\, \psi_{n+1} = a^\dag \psi_n.
\]
By applying the lowering operator $a$ to the above equation,
\[
\sqrt{n+1} a\psi_{n+1} = a a^\dag \psi_n = (\hat{N}+I) \psi_n = (n+1) \psi_n.
\]
Thus, $a \psi_{n+1} = \sqrt{n+1} \psi_n$, i.e.,
\[
a \psi_n = \sqrt{n} \psi_{n-1}.
\]

By applying \eqref{eq_eigenfunction-recursive} recursively,
\[
\psi_{n}(x) = \frac{1}{\sqrt{n!}}\,
(a^\dag)^n\psi_0(x),\quad n=1,2,3,\ldots. 
\]
The eigenfunctions can be expressed in terms of the $n^{th}$ order Hermite polynomials,
\[
\kappa_n(x) = (-1)^n e^{x^2} \frac{d^n}{dx^n} e^{-x^2}.
\]
By using Rodrigues formulae,
\begin{equation}\label{eq_eigenfunc-hermite}
\psi_n(x) = \frac{1}{\pi^{1/4} x_0^{n+1/2} \sqrt{2^n n!}} \kappa_n(x/x_0) e^{-x^2/(2 x_0^2)},\quad
x_0=\sqrt{\frac{\hbar}{m\omega}}.
\end{equation}

We summarize the most important relations in the following lemma.
\begin{lemma}
  The eigenvalue problem for the 1-D Schr\"odinger equation is
  \[
  e\psi = \frac{\hbar\omega}{2}\left( - x_0^2 \frac{\p^2\psi}{\p x^2} + \frac{x^2}{x_0^2}
  \psi\right) := \hat{H}\psi.
  \]
  Here, $x_0$ and $\omega$ are real constants, $e$ is the eigenvalue, $\psi$ is the eigenfunction, and $\hat{H}$
  is called the Hamiltonian operator. It can be factored into
  \[
  \hat{H} = \hbar\omega \left( a^\dag a + \frac{1}{2} \right),
  \]
  where $a$ and $a^\dag$ are called the lowering and raising operators, respectively,
  \[
  a = \frac{1}{\sqrt{2}}\left( \frac{x}{x_0} + x_0 \frac{\p}{\p x}\right),\quad
  %
  a^\dag = \frac{1}{\sqrt{2}}\left( \frac{x}{x_0} - x_0 \frac{\p}{\p x}\right),\quad
  x_0=\sqrt{\frac{\hbar}{m\omega}}.
  \]
  The smallest eigenvalue of $H$ and the corresponding normalized eigenfunction are
  \[
  e_0 = \frac{1}{2}\hbar\omega,\quad \psi_0(x) = \frac{e^{-x^2/(2 x_0^2)}}{\pi^{1/4} x_0^{1/2}}.
  \]
  The higher eigenvalues satisfy
  \[
  e_n = \hbar\omega\left(n + \frac{1}{2}\right),
  \]
  and the eigenfunctions are given by \eqref{eq_eigenfunc-hermite}. The normalized eigenfunctions
  satisfy the recursive relations
  \[
  a \psi_n = \sqrt{n} \psi_{n-1},\quad a^\dag \psi_n(x) = \sqrt{n+1}\, \psi_{n+1}.
  \]
\end{lemma}

From \eqref{eq_const-ratio}, the time dependence corresponding to the eigenfunction $\psi_n(x)$ with
eigenvalue $e_n$ satisfies 
\[
i\hbar \phi'_n = e_n \phi = \hbar\omega(n+1/2) \phi,
\]
which is solved by
\[
\phi_n(t) = c_n e^{-i(n+1/2)\omega t}.
\]
Thus, a general solution of the time-dependent Schr\"odinger equation can be written as an
eigenfunction expansion
\[
\Psi(x,t) = \sum_{n=0}^\infty c_n \psi_n(x) e^{-i(n+1/2)\omega t},
\]
where the coefficients $c_n$ are determined by the initial data.

\section{Matrix formulation}

\bibliographystyle{plain}
\bibliography{references}

\end{document}
